\documentclass{beamer}
\usepackage{setspace}
\usepackage{times}
\usepackage{tikz}
\usepackage{tkz-berge}
\usepackage{parskip}
\setlength{\parskip}{\smallskipamount} 
\usepackage{amsmath}
\usepackage{array}


\begin{document}


Let $d_1\ge2$, $d_2\ge2$, $k_1\ge1$, and $k_2\ge1q$. It follows from the fact that $A_2$ is a
$d_{2}$-basis for $\mathbb{Z}_{m_2}$ that
\[
q=\sum_{j=1}^{k_2}y_{j}a_{2j}+pm_2,
\]
where $y_{j}$'s are nonnegative integers with  $\sum_{j=1}^{k_{2}}y_{j}\le d_{2}$, and $p$ is an integer.
 Therefore,
\[
n\equiv\sum_{i=1}^{k_1}x_{i}a_{1i}+\sum_{j=1}^{k_2}y_{j}m_1a_{2j}\pmod{m_1m_2},
\]
where
\[
\sum_{i=1}^{k_{1}}x_{i}+\sum_{j=1}^{k_{2}}y_{j}\le d_{1}+d_{2}.
\]
This implies that n $\in d_$ be integers.  Then
\[
m(d_{1}+d_{2},k_1+k_2)\ge m(d_1,k_1)m(d_2,k_2).
\]

Let 
$A_s=\{0<a_{s1}<a_{s2}<\cdots<a_{sk_s}\}$ be a set of integers with
\[
m(d_s,A_s)=m(d_s,k_s)=m_s\qquad\hbox{for}\quad s=1,2.
\]
We may assume, without loss of generality, that $a_{sk_{s}}<m_{s}$ for $s=1,2$.
Define
\[
A=A_1\cup\{m_1a_{2j}\ |\ j=1,2,\ldots,k_2\}.
\]
Since $|A|=k_1+k_2$, we only need to prove that $A$ is a $(d_1+d_2)$-basis for $\mathbb{Z}_{m_1m_2}$.

 Let $n$ be any nonnegative integer. Since $A_1$ is an $d_{1}$-basis for $\mathbb{Z}_{m_1}$, we see that
\[
n\equiv \sum_{i=1}^{k_1}x_{i}a_{1i}\pmod{m_1},
\]
where $x_{i}$'s are nonnegative integers with  $\sum_{i=1}^{k_{1}}x_{i}\le d_{1}$.  Assume
\[
n=\sum_{i=1}^{k_1}x_{i}a_{1i}+qm_1
\]
for some integer $q$. It follows from the fact that $A_2$ is a
$d_{2}$-basis for $\mathbb{Z}_{m_2}$ that
\[
q=\sum_{j=1}^{k_2}y_{j}a_{2j}+pm_2,
\]
where $y_{j}$'s are nonnegative integers with  $\sum_{j=1}^{k_{2}}y_{j}\le d_{2}$, and $p$ is an integer.
 Therefore,
\[
n\equiv\sum_{i=1}^{k_1}x_{i}a_{1i}+\sum_{j=1}^{k_2}y_{j}m_1a_{2j}\pmod{m_1m_2},
\]
where
\[
\sum_{i=1}^{k_{1}}x_{i}+\sum_{j=1}^{k_{2}}y_{j}\le d_{1}+d_{2}.
\]
This implies that $n\in (d_1+d_2)A_{0}$, where $A_{0}=A\cup\{0\}$. Hence, $A$ is a $(d_{1}+d_{2})$-basis for $\mathbb{Z}_{m_1m_2}$. Therefore,
\[
m(d_{1},k_{1})m(d_{2},k_{2})=m_{1}m_{2}\le m(d_{1}+d_{2},k_{1}+k_{2}).
\]
The proof is complete.


\end{document}